pure_model/skeleton.lean
@@ -7,6 +7,9 @@ import LeanRV64DLEAN.RiscvExtras
 import LeanRV64DLEAN
 import LeanRV64DLEAN.pure_func
 
+set_option maxRecDepth 10_000
+set_option maxHeartbeats 1_000_000_000
+set_option match.ignoreUnusedAlts true
 
 open Functions
 open Retired
@@ -22,7 +25,6 @@ open PureFunctions
   wX_bits rd result
   pure RETIRE_SUCCESS -/
 
-
  -- regidx is of type BitVec
 def skeleton_binary  (rs2 : regidx) (rs1 : regidx) (rd : regidx) (execute_func : BitVec 64 → BitVec 64 → BitVec 64) : SailM Retired := do
   let rs1_val ← rX_bits rs1
@@ -37,84 +39,227 @@ def skeleton_unary (rs1 : regidx) (rd : regidx) (execute_func : BitVec 64 → Bi
   wX_bits rd result
   pure RETIRE_SUCCESS
 
-def skeleton_UTYPE (imm : BitVec 20) (rd : regidx) (op : uop) (execute_func : BitVec 20 → BitVec 64 → uop → BitVec 64) : SailM Retired := do
-  let pc ← get_arch_pc () -- TO DO READ IN THE PC , think of the effects
+def skeleton_UTYPE  (imm : BitVec 20) (rd : regidx) (op : uop) (execute_func : BitVec 20 → BitVec 64 → uop → BitVec 64) : SailM Retired := do
+  let pc ← get_arch_pc () -- states that I modelled this model like this bc its more uniform and neat but made the proof more compilcated
   let result := execute_func imm pc op
   wX_bits rd result
   pure RETIRE_SUCCESS
 
+-- introduced more skeletons depeending on whether pc was used or not
 
-theorem add_eq (Imm : BitVec 12) (rs1 : regidx) (rd : regidx) :
-    Functions.execute_ADDIW (imm) (rs1) (rd) = skeleton_unary rs1 rd (execute_ADDIW_pure64 imm) := by
-  unfold Functions.execute_ADDIW
-  unfold skeleton_unary
-  unfold execute_ADDIW_pure64
-  sorry
+def skeleton_UTYPE_AUIPC  (imm : BitVec 20) (rd : regidx) (execute_func : BitVec 20 → BitVec 64 → BitVec 64) : SailM Retired := do
+  let pc ← get_arch_pc (); -- TO DO READ IN THE PC , think of the effects
+  let result := execute_func imm pc
+  wX_bits rd result
+  pure RETIRE_SUCCESS
+
+def skeleton_UTYPE_LUI  (imm : BitVec 20) (rd : regidx) (execute_func : BitVec 20 → BitVec 64 → BitVec 64) : SailM Retired := do
+  let result := execute_func imm 0#64
+  wX_bits rd result
+  pure RETIRE_SUCCESS
 
 
-theorem utype_eq (imm : (BitVec 20)) (rd : regidx) (op : uop) :
-    Functions.execute_UTYPE imm rd op = skeleton_UTYPE imm rd op (execute_UTYPE_pure64) := by
-  sorry
+theorem add_eq (imm : BitVec 12) (rs1 : regidx) (rd : regidx) :
+    Functions.execute_ADDIW (imm) (rs1) (rd)
+    = skeleton_unary rs1 rd (execute_ADDIW_pure64 imm)
+  := by
+  unfold Functions.execute_ADDIW skeleton_unary execute_ADDIW_pure64
+  rfl
+
+-- case destinction on the type of uop operation
+theorem utype_eq_LUI (imm : (BitVec 20)) (rd : regidx):
+    Functions.execute_UTYPE imm rd (uop.RISCV_LUI)
+    =
+    skeleton_UTYPE_LUI imm rd (fun imm pc => execute_UTYPE_pure64 imm pc (uop.RISCV_LUI) )
+  := by
+  unfold Functions.execute_UTYPE skeleton_UTYPE_LUI execute_UTYPE_pure64
+  simp only [Nat.reduceAdd, BitVec.ofNat_eq_ofNat, bind_pure_comp, pure_bind]
+
+theorem utype_eq_AUIPC (imm : (BitVec 20)) (rd : regidx):
+  Functions.execute_UTYPE imm rd (uop.RISCV_AUIPC)
+    = skeleton_UTYPE_AUIPC  imm rd (fun imm pc => execute_UTYPE_pure64 imm pc uop.RISCV_AUIPC)
+  := by
+    unfold Functions.execute_UTYPE skeleton_UTYPE_AUIPC execute_UTYPE_pure64
+    simp only [Nat.reducePow, Nat.reduceMul, Nat.reduceAdd, BitVec.ofNat_eq_ofNat, bind_pure_comp,
+      bind_map_left, BitVec.add_eq]
+
+/-
+theorem ignore_pc (x: SailM (BitVec 64)) :
+  let pc ← get_arch_pc ();
+  (fun a => RETIRE_SUCCESS) <$> wX_bits rd (sign_extend ((imm : (BitVec 20))  ++ 0#12)) =
+  (fun a => RETIRE_SUCCESS) <$> wX_bits rd (sign_extend ((imm : (BitVec 20)) ++ 0#12)) :=
+    by simp
+-/
+--#print StateT
+--#check (Functions.execute_UTYPE ?imm ?rd ?f : _ → _)
+
+--def SailM := Nat → Nat
+
+--def f : NatFun :=
+  --fun a => a
+--(h: Register.PC = Some s ) (h: Register.PC == Some s )
+
+theorem utype_eq (imm : (BitVec 20)) (rd : regidx) (op : uop) (h_pc : s.regs.get? Register.PC = some valt):
+    Functions.execute_UTYPE imm rd op s
+     = skeleton_UTYPE imm rd op (execute_UTYPE_pure64) s
+  := by
+  unfold Functions.execute_UTYPE skeleton_UTYPE execute_UTYPE_pure64
+  cases op
+  ·
+    simp only [Nat.reduceAdd, BitVec.ofNat_eq_ofNat, bind_pure_comp, pure_bind, Nat.reducePow,
+      Nat.reduceMul]
+    simp [get_arch_pc, readReg, PreSail.readReg, Monad.toBind, EStateM.instMonad, EStateM.map,
+      EStateM.bind, get, getThe, MonadStateOf.get, EStateM.get]
+    cases hs : s.regs.get? Register.PC
+    · rw [hs] at h_pc
+      contradiction
+    · simp only
+      rfl
+  ·
+   simp only [Nat.reducePow, Nat.reduceMul, Nat.reduceAdd, BitVec.ofNat_eq_ofNat, bind_pure_comp,
+     bind_map_left, BitVec.add_eq]
 
 theorem shiftiwop_eq (shamt : (BitVec 5)) (rs1 : regidx) (rd : regidx) (op : sopw) :
-    Functions.execute_SHIFTIWOP (shamt) (rs1) (rd) (op) = skeleton_unary rs1 rd (fun val1 => PureFunctions.execute_SHIFTIWOP_pure64 shamt op val1) := by
-  sorry
+    Functions.execute_SHIFTIWOP (shamt) (rs1) (rd) (op)
+      = skeleton_unary rs1 rd (fun val1 => PureFunctions.execute_SHIFTIWOP_pure64 shamt op val1)
+  := by
+  unfold Functions.execute_SHIFTIWOP skeleton_unary execute_SHIFTIWOP_pure64
+  rfl
 
 theorem shiftiop_eq (shamt : (BitVec 6)) (op : sop) (rs1 : regidx) (rd : regidx) :
-    Functions.execute_SHIFTIOP (shamt) (rs1) (rd) (op) = skeleton_unary rs1 rd (fun val1 => execute_SHIFTIOP_pure64 shamt op val1)  := by
-  sorry
+    Functions.execute_SHIFTIOP (shamt) (rs1) (rd) (op)
+      = skeleton_unary rs1 rd (fun val1 => PureFunctions.execute_SHIFTIOP_pure64 shamt op val1)
+  := by
+  unfold Functions.execute_SHIFTIOP skeleton_unary execute_SHIFTIOP_pure64
+  cases op
+  <;> simp
 
 theorem rtypew_eq (rs2 : regidx) (rs1 : regidx) (rd : regidx) (op : ropw) :
-    Functions.execute_RTYPEW (rs2) (rs1) (rd) (op) = skeleton_binary rs2 rs1 rd (fun val1 val2 => execute_RTYPEW_pure64 op val2 val1) := by -- attention_ ordering of arguements
-  sorry
+    Functions.execute_RTYPEW (rs2) (rs1) (rd) (op)
+      = skeleton_binary rs2 rs1 rd (fun val1 val2 => execute_RTYPEW_pure64 op val2 val1)
+  := by -- attention_ ordering of arguements
+  unfold Functions.execute_RTYPEW skeleton_binary execute_RTYPEW_pure64
+  rfl
 
-theorem rtype_eq (rs2 : regidx) (rs1 : regidx) (rd : (regidx)) (op : rop) :
-    Functions.execute_RTYPE (rs2) (rs1) (rd) (op) = skeleton_binary rs2 rs1 rd (fun val1 val2 => execute_RTYPE_pure64 op val2 val1) := by
-  sorry
+theorem rtype_eq (rs2 : regidx) (rs1 : regidx) (rd : regidx) (op : rop) :
+    Functions.execute_RTYPE (rs2) (rs1) (rd) (op)
+      = skeleton_binary rs2 rs1 rd (fun val1 val2 => execute_RTYPE_pure64 op val2 val1)
+  := by
+  unfold Functions.execute_RTYPE skeleton_binary execute_RTYPE_pure64
+  simp
+  cases op
+  <;> simp
+
 
 theorem remw_eq (rs2 : regidx) (rs1 : regidx) (rd : regidx) (s : Bool) :
-    Functions.execute_REMW (rs2) (rs1) (rd) (s) = skeleton_binary rs2 rs1 rd (fun val1 val2 => execute_REMW_pure64 s val2 val1) := by
-  sorry
+    Functions.execute_REMW (rs2) (rs1) (rd) (s)
+      = skeleton_binary rs2 rs1 rd (fun val1 val2 => execute_REMW_pure64 s val2 val1)
+  := by
+  unfold Functions.execute_REMW skeleton_binary execute_REMW_pure64
+  rfl
 
 theorem rem_eq (rs2 : regidx) (rs1 : regidx) (rd : regidx) (s : Bool) :
-    Functions.execute_REM (rs2) (rs1) (rd) (s) = skeleton_binary rs2 rs1 rd (fun val1 val2 => execute_REM_pure64 s val2 val1) := by
-  sorry
+    Functions.execute_REM (rs2) (rs1) (rd) (s)
+      = skeleton_binary rs2 rs1 rd (fun val1 val2 => execute_REM_pure64 s val2 val1)
+  := by
+  unfold Functions.execute_REM skeleton_binary execute_REM_pure64
+  rfl
 
-theorem mulw_eq (rs2_val : (BitVec 64)) (rs1_val : (BitVec 64)) :
-    Functions.execute_MULW (rs2) (rs1) (rd) = skeleton_binary rs2 rs1 rd (fun val1 val2 => execute_MULW_pure64 val2 val1) := by
-  sorry
+theorem mulw_eq (rs2 : regidx) (rs1 : regidx) (rd : regidx) :
+    Functions.execute_MULW (rs2) (rs1) (rd)
+      = skeleton_binary rs2 rs1 rd (fun val1 val2 => execute_MULW_pure64 val2 val1)
+  := by
+  unfold Functions.execute_MULW skeleton_binary execute_MULW_pure64
+  rfl
 
 theorem mul_eq (rs2 : regidx) (rs1 : regidx) (rd : regidx) (mul_op : mul_op) :
-    Functions.execute_MUL (rs2 ) (rs1) (rd) (mul_op) = skeleton_binary rs2 rs1 rd (fun val1 val2 => execute_MUL_pure64 mul_op val2 val1) := by
-  sorry
+    Functions.execute_MUL (rs2 ) (rs1) (rd) (mul_op)
+      = skeleton_binary rs2 rs1 rd (fun val1 val2 => execute_MUL_pure64 mul_op val2 val1)
+  := by
+  unfold Functions.execute_MUL skeleton_binary execute_MUL_pure64
+  rfl
 
 theorem divw_eq (rs2 : regidx) (rs1 : regidx) (rd : regidx) (s : Bool) :
-    Functions.execute_DIVW (rs2 ) (rs1) (rd) (s) = skeleton_binary rs2 rs1 rd (fun val1 val2 => execute_DIVW_pure64 s val2 val1) := by
-  sorry
+    Functions.execute_DIVW (rs2 ) (rs1) (rd) (s)
+      = skeleton_binary rs2 rs1 rd (fun val1 val2 => execute_DIVW_pure64 s val2 val1)
+  := by
+  unfold Functions.execute_DIVW skeleton_binary execute_DIVW_pure64
+  rfl
+
 
 theorem div_eq (rs2 : regidx) (rs1 : regidx) (rd : regidx) (s : Bool) :
-    Functions.execute_DIV (rs2) (rs1) (rd) (s) = skeleton_binary rs2 rs1 rd (fun val1 val2 => execute_DIV_pure64 s val2 val1) := by
-  sorry
+    Functions.execute_DIV (rs2) (rs1) (rd) (s)
+      = skeleton_binary rs2 rs1 rd (fun val1 val2 => execute_DIV_pure64 s val2 val1)
+  := by
+  unfold Functions.execute_DIV skeleton_binary execute_DIV_pure64
+  rfl
 
 theorem itype_eq (imm : (BitVec 12)) (rs1 : regidx) (rd : regidx) (op : iop) :
-    Functions.execute_ITYPE (imm) (rs1) (rd) (op) = skeleton_unary rs1 rd (fun val1 => execute_ITYPE_pure64 imm val1 op) := by
-  sorry
+    Functions.execute_ITYPE (imm) (rs1) (rd) (op)
+      = skeleton_unary rs1 rd (fun val1 => execute_ITYPE_pure64 imm val1 op)
+  := by
+  unfold Functions.execute_ITYPE skeleton_unary execute_ITYPE_pure64
+  · cases op
+  <;> simp
 
 theorem zicond_rtype_eq (arg0 : regidx) (arg1 : regidx) (arg2 : regidx) (arg3 : zicondop) :
-    Functions.execute_ZICOND_RTYPE arg0 arg1 arg2 arg3 = skeleton_binary arg0 arg1 arg2 (fun val1 val2 => execute_ZICOND_RTYPE_pure64 val2 val1 arg3) := by
-  sorry
+    Functions.execute_ZICOND_RTYPE arg0 arg1 arg2 arg3
+      = skeleton_binary arg0 arg1 arg2 (fun val1 val2 => execute_ZICOND_RTYPE_pure64 val2 val1 arg3)
+  := by
+  unfold Functions.execute_ZICOND_RTYPE skeleton_binary execute_ZICOND_RTYPE_pure64
+  · cases arg3
+  <;> simp
 
 theorem zbs_rytpe_eq (rs2 : regidx) (rs1 : regidx) (rd : regidx) (op : brop_zbs) :
-    Functions.execute_ZBS_RTYPE rs2 rs1 rd op = skeleton_binary rs2 rs1 rd (fun val1 val2 => execute_ZBS_RTYPE_pure64 val2 val1 op) := by
-  sorry
+    Functions.execute_ZBS_RTYPE rs2 rs1 rd op
+      = skeleton_binary rs2 rs1 rd (fun val1 val2 => execute_ZBS_RTYPE_pure64 val2 val1 op)
+  := by
+  unfold Functions.execute_ZBS_RTYPE skeleton_binary execute_ZBS_RTYPE_pure64
+  rfl
 
 theorem zbs_iop_eq (shamt : (BitVec 6)) (rs1 : regidx) (rd : regidx) (op : biop_zbs) :
-    execute_ZBS_IOP (shamt ) (rs1) (rd) (op) = skeleton_unary rs1 rd (fun val1 => execute_ZBS_IOP_pure64 shamt val1 op)  :=by
-  sorry
+    execute_ZBS_IOP (shamt ) (rs1) (rd) (op) = skeleton_unary rs1 rd (fun val1 => execute_ZBS_IOP_pure64 shamt val1 op)
+  := by
+  unfold Functions.execute_ZBS_IOP skeleton_unary execute_ZBS_IOP_pure64
+  rfl
+
+-- to do ZBKS for crypto
+
+theorem zbb_rtypew_eq (rs2 : regidx) (rs1 : regidx) (rd : regidx) (op : bropw_zbb) :
+    Functions.execute_ZBB_RTYPEW (rs2) (rs1) (rd) (op)
+    = skeleton_binary rs2 rs1 rd (fun val1 val2 => execute_ZBB_RTYPEW_pure64 val2 val1 op)
+  := by
+  unfold Functions.execute_ZBB_RTYPEW skeleton_binary execute_ZBB_RTYPEW_pure64
+  rfl
 
 
--- TO DO ZICOND and ZBB RytPEW
+theorem zbb_extop_eq (rs1 : regidx) (rd : regidx) (op : extop_zbb)  :
+    Functions.execute_ZBB_EXTOP (rs1) (rd) (op)
+    = skeleton_unary rs1 rd (fun val1 => execute_ZBB_EXTOP_pure64 val1 op)
+  := by
+  unfold Functions.execute_ZBB_EXTOP skeleton_unary execute_ZBB_EXTOP_pure64
+  rfl
 
+theorem zba_rtypeuw_eq (rs2 : regidx) (rs1 : regidx) (rd : regidx) (op : bropw_zba)  :
+    Functions.execute_ZBA_RTYPEUW (rs2) (rs1) (rd) (op)
+    = skeleton_binary rs2 rs1 rd (fun val1 val2 => execute_ZBA_RTYPEUW_pure64 val2 val1 op)
+  := by
+  unfold Functions.execute_ZBA_RTYPEUW skeleton_binary execute_ZBA_RTYPEUW_pure64
+  rfl
+
+theorem zba_rtype_eq (rs2 : regidx) (rs1 : regidx) (rd : regidx) (op : brop_zba)  :
+    Functions.execute_ZBA_RTYPE (rs2) (rs1) (rd) (op)
+    = skeleton_binary rs2 rs1 rd (fun val1 val2 => execute_ZBA_RTYPE_pure64 val2 val1 op)
+  := by
+  unfold Functions.execute_ZBA_RTYPE skeleton_binary execute_ZBA_RTYPE_pure64
+  rfl
+
+
+example (p q : Prop) : p ∨ q → q ∨ p := by
+  intro h
+  cases h with
+  | inr hq => apply Or.inl; exact hq
+  | inl hp => apply Or.inr; exact hp
 
 
 
